Prove the soundness of the compilation pipeline given arbitrary optimization heuristics

fiat2/src/fiat2/OptimizeAnno.v
@@ -1,12 +1,13 @@
 Require Import fiat2.Language fiat2.Interpret fiat2.Value fiat2.TypeSystem fiat2.TypeSound fiat2.IndexInterface
   fiat2.CollectionTransf fiat2.DictIndexImpl fiat2.SumAgg fiat2.MinAgg fiat2.BitmapIndex fiat2.TransfUtils fiat2.RelTransf fiat2.IndexTransf fiat2.TransfSound fiat2.Utils fiat2.Substitute.
 Require Import coqutil.Map.Interface coqutil.Map.SortedListString coqutil.Word.Interface coqutil.Datatypes.Result.
-From Stdlib Require Import List String ZArith.
+From Stdlib Require Import List String ZArith Permutation.
 Import ListNotations.
 
 Variant basic_transf :=
-  | ToJoin
   | ToFilter
+  | ToProj
+  | ToJoin
   | FilterPushdown
   | AnnotateCollection
   | PushdownCollection.
@@ -34,8 +35,8 @@ Section WithConcreteMaps.
   Instance clocals_ok : map.ok clocals := SortedListString.ok _.
 
   Section CommonPipelineParts.
-    Context (sum_agg_attr : string).
     Context (tag tag' : string).
+    Context (sum_agg_attr : string).
 
     Definition sum_agg_wf := (SumAgg.idx_wf (locals:=clocals) "hole" sum_agg_attr "x").
     Instance csum_agg : IndexInterface.index := (sum_agg "hole" sum_agg_attr "x").
@@ -227,4 +228,345 @@ end.
     intros. apply mk_idxs_ok in H; intuition idtac.
     apply compo_idx_ok; auto.
   Qed.
+
+  Definition to_proj_transf := fold_command id to_proj_head.
+  Definition to_filter_transf := fold_command id to_filter_head.
+  Definition to_join_transf := fold_command id to_join_head.
+  Definition annotate_collection_transf := fold_command id annotate_collection.
+  Definition push_down_collection_transf := fold_command id push_down_collection.
+  Definition filter_pushdown_transf := fold_command id filter_pushdown_head.
+
+  Definition mk_basic_transf (f : basic_transf) : command -> command :=
+    match f with
+    | ToFilter => to_filter_transf
+    | ToProj => to_proj_transf
+    | ToJoin => to_join_transf
+    | FilterPushdown => filter_pushdown_transf
+    | AnnotateCollection => annotate_collection_transf
+    | PushdownCollection => push_down_collection_transf
+    end.
+
+  Definition compose_basic_transfs : list (command -> command) -> command -> command :=
+    fold_right Basics.compose id.
+
+  Definition mk_idx_use_transfs (l : list (string -> command -> command)) : string -> command -> command :=
+    fun tbl => fold_right (fun f g => Basics.compose (f tbl) g) id l.
+
+  Definition mk_idx_related_transfs (idx : IndexInterface.index) (f : string -> command -> command) :
+    ctenv -> ctenv -> command -> command :=
+    apply_idx_related_transfs (idx:=idx) "id_tag" "aux_tag" f.
+
+  Fixpoint apply_below_n_letmuts (n : nat) (f : ctenv -> ctenv -> command -> command) :
+    ctenv -> ctenv -> command -> command :=
+    match n with
+    | O => f
+    | S n => apply_below_n_letmuts n (apply_below_letmut f)
+    end.
+
+  Fixpoint compose_all_idx_transfs (n : nat) (l : list (ctenv -> ctenv -> command -> command)) :
+    ctenv -> ctenv -> command -> command :=
+    match l with
+    | [] => fun _ _ => id
+    | f :: l =>
+        fun Gstore Genv =>
+          Basics.compose (apply_below_n_letmuts n f Gstore Genv) (compose_all_idx_transfs (S n) l Gstore Genv)
+    end.
+
+  Definition apply_all_transfs (reps : nat) (fs : list basic_transf) (icss : list (list index_choice)) (Gstore Genv : ctenv) :=
+    let idx_transfs :=
+      map (fun ics =>
+             let '(idxs, transfs, _) := mk_idxs O reps ics in
+             let cidx := mk_compo_idx idxs in
+             let idx_use_transfs := mk_idx_use_transfs transfs in
+             mk_idx_related_transfs cidx idx_use_transfs) icss in
+    (Basics.compose (compose_all_idx_transfs O idx_transfs Gstore Genv) (compose_basic_transfs (map mk_basic_transf fs))).
+
+  Definition apply_optimize_anno (ac : anno_command) (Gstore Genv : ctenv) :=
+    match ac with
+    | AC fs icss c =>
+        apply_all_transfs 10000 fs icss Gstore Genv c
+    end.
+
+  Lemma id_transf_sound : transf_sound (locals:=clocals) (fun _ _ => id).
+  Proof.
+    unfold transf_sound; intuition auto.
+  Qed.
+
+  Hint Resolve id_transf_sound : transf_hints.
+
+  Lemma compose_basic_transfs_sound : forall fs,
+      transf_sound (locals := clocals)
+        (fun _ _ : ctenv =>
+           compose_basic_transfs (map mk_basic_transf fs)).
+  Proof.
+    induction fs; cbn; auto with transf_hints.
+    apply_transf_sound_lemmas; auto.
+    destruct a; eauto with transf_hints.
+  Qed.
+
+  Lemma apply_below_n_letmuts_sound : forall n f,
+      transf_sound (locals:=clocals) f ->
+      transf_sound (locals:=clocals) (apply_below_n_letmuts n f).
+  Proof.
+    induction n; cbn; auto; intros.
+    apply IHn. apply_transf_sound_lemmas.
+    assumption.
+  Qed.
+
+  Lemma compose_all_idx_transfs_sound : forall l n,
+      Forall (transf_sound (locals:=clocals)) l ->
+      transf_sound (locals:=clocals) (compose_all_idx_transfs n l).
+  Proof.
+    induction l; cbn; intros; auto with transf_hints.
+    apply_transf_sound_lemmas; invert_Forall; auto.
+    apply apply_below_n_letmuts_sound.
+    assumption.
+  Qed.
+
+  Lemma id_aug_transf_sound : forall is_tbl_ty aux_ty (aux_wf : value -> Prop),
+      aug_transf_sound is_tbl_ty aux_ty aux_wf (fun _ => id).
+  Proof.
+    unfold aug_transf_sound; cbn; auto.
+  Qed.
+
+  Lemma aug_transf_sound_fold_compose : forall is_tbl_ty aux_ty aux_wf transfs,
+      Forall (aug_transf_sound (locals:=clocals) is_tbl_ty aux_ty aux_wf) transfs ->
+    aug_transf_sound is_tbl_ty aux_ty aux_wf
+    (fun tbl : string =>
+       fold_right
+         (fun f g => Basics.compose (f tbl) g)
+         id transfs).
+  Proof.
+    induction transfs; cbn; intros.
+    1: apply id_aug_transf_sound.
+    invert_Forall.
+    apply_transf_sound_lemmas; auto.
+  Qed.
+
+  Ltac apply_in_nil :=
+    lazymatch goal with
+      H: In _ [] |- _ =>
+        apply in_nil in H; intuition fail
+    end.
+
+  Ltac apply_incl_cons_inv :=
+    lazymatch goal with
+      H: incl (_ :: _) _ |- _ =>
+        apply incl_cons_inv in H; intuition idtac
+    end.
+
+  Lemma map_fst_map_fst : forall A B C D (l : list (A * B * C)) (f : B -> D),
+      map fst (map (fun '(a, b, _) => (a, f b)) l) = map fst (map fst l).
+  Proof.
+    induction l; cbn; auto; intros.
+    repeat case_match; cbn; f_equal.
+    auto.
+  Qed.
+
+  Ltac apply_in_map :=
+    lazymatch goal with
+      H: In _ ?l |- In _ (map ?g ?l) =>
+        apply in_map with (f:=g) in H
+    end.
+
+  Ltac apply_in_map_with_tag :=
+    lazymatch goal with
+      H: In (?tag, _, _) ?l |- In (?tag, _) (map ?g ?l) =>
+        apply in_map with (f:=g) in H
+    end.
+
+  Ltac prove_aux_ty_for_idx :=
+    lazymatch goal with
+      |- aux_ty_for_idx _ _ _ _ _ =>
+        unfold aux_ty_for_idx;
+        intros; cbn; intuition idtac;
+        erewrite NoDup_Permutation_access_record;
+        try apply Permutation.Permutation_sym, Permuted_record_sort
+    end.
+
+  Ltac prove_access_record_idx_ty :=
+    apply NoDup_In_access_record;
+    [ rewrite map_fst_map_fst; assumption
+    | apply_in_map_with_tag; auto ].
+
+  Ltac prove_NoDup_map_fst_sort_map :=
+    eapply Permutation_NoDup; try eassumption;
+    eapply perm_trans;
+    [ | eapply Permutation_map, Permuted_record_sort ];
+    rewrite map_fst_map_fst; auto.
+
+  Ltac prove_In_map_fst_sort_map :=
+    eapply Permutation_in;
+    [ apply Permutation_map, Permuted_record_sort | ];
+    rewrite map_map;
+    apply_in_map; cbn in *;
+    try lazymatch goal with
+      | H:In (?tag, _, _) ?l |- In ?tag (map ?g ?l) => apply in_map with (f := g) in H
+      end;
+    assumption.
+
+  Ltac prove_is_tbl_ty :=
+    unfold compo_is_tbl_ty; intros;
+    rewrite forallb_forall in *;
+    repeat lazymatch goal with
+      H: forall _, In _ _ -> _, H': In _ _ |- _ =>
+    apply H in H'
+  end; assumption.
+
+  Ltac prove_idx_wf :=
+    unfold aux_wf, aux_wf_for_idx; intros;
+    do 4 (case_match; intuition idtac);
+    unfold compo_idx_wf in *;
+    repeat lazymatch goal with
+    | H:Forall _ ?l, H':In _ ?l |- _ =>
+        let H_new := fresh "H_new" in
+        eapply List.Forall_In in H as H_new; eauto; clear H'
+    end;
+    repeat destruct_match_hyp; intuition idtac;
+    repeat invert_pair; rewrite_l_to_r; try eassumption.
+
+  Lemma mk_idx_sound : forall ic init_tag reps idxs transfs next_tag f,
+      (idxs, transfs, next_tag) = mk_idx init_tag reps ic ->
+      In f transfs ->
+      forall l,
+        incl idxs l ->
+        NoDup (map fst (map fst l)) ->
+        @aug_transf_sound width word ctenv clocals (@IndexInterface.is_tbl_ty (mk_compo_idx l))
+          (@aux_ty (mk_compo_idx l) "id_tag" "aux_tag") (@aux_wf width word (@compo_idx_wf width word l) "id_tag" "aux_tag") f.
+  Proof.
+    destruct ic; cbn; intros; invert_pair; repeat apply_incl_cons_inv.
+    1:{ repeat destruct_In; try apply_in_nil; repeat apply_transf_sound_lemmas.
+        1:{ eapply sum_to_agg_lookup_head_sound; auto using ctenv_ok, clocals_ok.
+            1: prove_aux_ty_for_idx;
+            [ prove_access_record_idx_ty
+            | prove_NoDup_map_fst_sort_map
+            | prove_In_map_fst_sort_map ].
+            1: prove_is_tbl_ty.
+            1: prove_idx_wf. }
+        1:{ apply expr_transf_sound__expr_aug_transf_sound.
+            eapply cons_to_add_head_sound. } }
+    1:{ repeat destruct_In; try apply_in_nil; repeat apply_transf_sound_lemmas.
+        1:{ eapply min_to_agg_lookup_head_sound; auto using ctenv_ok, clocals_ok.
+            1: prove_aux_ty_for_idx;
+            [ prove_access_record_idx_ty
+            | prove_NoDup_map_fst_sort_map
+            | prove_In_map_fst_sort_map ].
+            1: prove_is_tbl_ty.
+            1: prove_idx_wf. }
+        1:{ apply expr_transf_sound__expr_aug_transf_sound.
+            eapply cons_to_min_head_sound. } }
+    1:{ repeat destruct_In; try apply_in_nil; repeat apply_transf_sound_lemmas.
+        1:{ eapply eq_filter_to_lookup_head_sound; auto using ctenv_ok, clocals_ok.
+            1:{ rewrite is_NoDup_to_transparent.
+                instantiate(3:="tup"). instantiate (2:="acc"). instantiate (1:="x").
+                cbn; intuition discriminate. }
+            1: prove_aux_ty_for_idx;
+            [ prove_access_record_idx_ty
+            | prove_NoDup_map_fst_sort_map
+            | prove_In_map_fst_sort_map ].
+            1: prove_is_tbl_ty.
+            1: prove_idx_wf. }
+        1:{ eapply use_idx_head_sound; eauto with transf_hints.
+            1:{ rewrite is_NoDup_to_transparent.
+                instantiate(3:="tup"). instantiate (2:="acc"). instantiate (1:="x").
+                eauto with transf_hints. }
+            1: prove_aux_ty_for_idx;
+            [ prove_access_record_idx_ty
+            | prove_NoDup_map_fst_sort_map
+            | prove_In_map_fst_sort_map ].
+            1: prove_is_tbl_ty.
+            1: prove_idx_wf. }
+        1:{ apply expr_transf_sound__expr_aug_transf_sound.
+            eapply cons_to_insert_head_sound;
+              eauto with transf_hints. } }
+    1:{ repeat destruct_In; try apply_in_nil; repeat apply_transf_sound_lemmas.
+        1:{ eapply filter_to_bitmap_lookup_head_sound;
+              eauto with transf_hints.
+            1:{ rewrite is_NoDup_to_transparent.
+                instantiate(2:="pk_tup"). instantiate (1:="pk_acc").
+                eauto with transf_hints. }
+            1,2: prove_aux_ty_for_idx;
+            [ prove_access_record_idx_ty
+            | prove_NoDup_map_fst_sort_map
+            | prove_In_map_fst_sort_map ].
+            1,2: prove_is_tbl_ty.
+            1,2: prove_idx_wf; instantiate(1:="hole"); auto. }
+        1:{ eapply use_bitmap_head_sound;
+              eauto with transf_hints.
+            1: prove_aux_ty_for_idx;
+            [ prove_access_record_idx_ty
+            | prove_NoDup_map_fst_sort_map
+            | prove_In_map_fst_sort_map ].
+            1: prove_is_tbl_ty.
+            1: prove_idx_wf. }
+        1:{ apply expr_transf_sound__expr_aug_transf_sound.
+            eapply cons_to_bitmap_update_head_sound. }
+        1:{ eapply use_pk_idx_head_sound;
+            eauto with transf_hints.
+            1:{ instantiate(2:="pk_tup"); instantiate(1:="pk_acc");
+                eauto with transf_hints. }
+            1: prove_aux_ty_for_idx;
+            [ prove_access_record_idx_ty
+            | prove_NoDup_map_fst_sort_map
+            | prove_In_map_fst_sort_map ].
+            1: prove_is_tbl_ty.
+            1: prove_idx_wf; instantiate (1:="hole"); assumption. }
+        1:{ apply expr_transf_sound__expr_aug_transf_sound.
+            apply cons_to_pk_idx_update_head_sound. } }
+  Qed.
+
+  Lemma mk_idxs_mk_idx : forall ics init_tag reps idxs transfs next_tag f,
+      (idxs, transfs, next_tag) = mk_idxs init_tag reps ics ->
+      In f transfs ->
+      exists ic init_tag' reps idxs' transfs' next_tag',
+        In ic ics /\
+          (idxs', transfs', next_tag') = mk_idx init_tag' reps ic /\
+          incl idxs' idxs /\
+          In f transfs'.
+  Proof.
+    induction ics; cbn; intros.
+    1:{ invert_pair. apply_in_nil. }
+    1:{ repeat destruct_match_hyp. invert_pair.
+        rewrite in_app_iff in *; intuition idtac.
+        1:{ repeat eexists; eauto using incl_appl, incl_refl. }
+        1:{ eapply IHics in H; eauto.
+            repeat destruct_exists; intuition idtac.
+            repeat eexists; try eassumption;
+              intuition auto using incl_appr. } }
+  Qed.
+
+  Lemma mk_idx_related_transfs_sound : forall ics idxs transfs n init_tag reps,
+      (idxs, transfs, n) = mk_idxs init_tag reps ics ->
+      transf_sound (locals:=clocals) (mk_idx_related_transfs (mk_compo_idx idxs) (mk_idx_use_transfs transfs)).
+  Proof.
+    unfold mk_idx_related_transfs, mk_idx_use_transfs.
+    intros.
+    eapply apply_idx_related_transfs_sound.
+    1: discriminate.
+    apply aug_transf_sound_fold_compose.
+    instantiate (1:=compo_idx_wf idxs).
+    rewrite Forall_forall; intros.
+    eapply mk_idxs_mk_idx in H0; eauto.
+    repeat destruct_exists; intuition idtac.
+    eapply mk_idx_sound; eauto.
+    eapply mk_idxs_ok; eauto.
+    Unshelve.
+    all: eauto with transf_hints.
+    eapply mk_compo_idx_ok; eauto.
+  Qed.
+
+  Theorem apply_all_transfs_sound : forall reps fs icss,
+      transf_sound (locals:=clocals) (apply_all_transfs reps fs icss).
+  Proof.
+    unfold apply_all_transfs; intros.
+    apply transf_sound_compose.
+    2: apply compose_basic_transfs_sound.
+    apply compose_all_idx_transfs_sound.
+    rewrite Forall_forall; intros.
+    rewrite in_map_iff in *.
+    destruct_exists; intuition idtac.
+    repeat destruct_match_hyp. subst.
+    eapply mk_idx_related_transfs_sound; eauto.
+  Qed.
+
 End WithConcreteMaps.
